lib/coq/todo.md
@@ -13,6 +13,3 @@
 - Reusing essentially the [mon] monad from CompCert that is more or less [FreshT fail]
 - Question of initial seed: should be fine to just use 0 for us
 - Question of tracking ident to source name: duplicate locally [mon] with an extended [trail] field?
-
-
-
